6_finished

1_SetTheory/6_Order/Solution.lean
@@ -7043,7 +7043,7 @@ theorem lin_latt : ∀ 𝓐, (LinOrd 𝓐) → (Latt 𝓐) :=
       )
 
 
-def is_well_order 𝓐 := (LinOrd 𝓐) ∧ ∀ X, (X ≠ ∅) → (X ⊆ setPO(𝓐)) → (𝓐 MinExi X)
+def is_well_order 𝓐 := (LinOrd 𝓐) ∧ ∀ X, (X ⊆ setPO(𝓐)) → (X ≠ ∅) → (𝓐 MinExi X)
 syntax "WellOrd" term : term
 macro_rules
 | `(WellOrd $𝓐) => `(is_well_order $𝓐)
@@ -9124,7 +9124,61 @@ theorem poiso_latt : ∀ 𝓐 𝓑, (𝓐 P≃O 𝓑) → ((Latt 𝓐) ↔ (Latt
       )
 
 
-theorem poiso_complatt : ∀ 𝓐 𝓑, (𝓐 P≃O 𝓑) → ((CompLatt 𝓐) ↔ (CompLatt 𝓑)) := sorry
+theorem poiso_subset_prop (φ : Set → Set → Prop) :
+(∀ 𝓐 𝓑 f X, (X ⊆ setPO(𝓐)) → (f PO_ISO_PO 𝓐 To 𝓑) → ((φ 𝓐 X) ↔ (φ 𝓑 (f.[X])))) →
+(∀ 𝓐 𝓑, (𝓐 P≃O 𝓑) → ((∀ X, (X ⊆ setPO(𝓐)) → (φ 𝓐 X)) ↔ (∀ X, (X ⊆ setPO(𝓑)) → (φ 𝓑 X)))) :=
+  fun (hProp) =>
+    fun (𝓐 𝓑 hPO) =>
+      Exists.elim (And.right (And.right (hPO))) (
+        fun (f) =>
+          fun (hf) =>
+            let hfbij := And.left hf
+            let hfunc := And.left hfbij
+            let hfinvbij := bijection_inv_mp f (setPO(𝓐)) (setPO(𝓑)) hfbij
+            let hfinvfunc := And.left hfinvbij
+            let hfinvpfunc := And.left hfinvfunc
+            let hiso := And.intro (And.left (hPO)) (And.intro (And.left (And.right hPO)) (hf))
+            Iff.intro
+            (
+              fun (h𝓐X) =>
+                fun (X) =>
+                  fun (hX : X ⊆ setPO(𝓑)) =>
+                    let v₀ := specification_set_subset (fun (b) => ∃ a ∈ X; (a . (f⁻¹) . b)) (rng (f⁻¹))
+                    let v₁ := rng_partial_function (f⁻¹) (setPO(𝓑)) (setPO(𝓐)) hfinvpfunc
+                    let v₂ := subset_trans (f⁻¹.[X]) (rng (f⁻¹)) (setPO(𝓐)) v₀ v₁
+                    let u₀ := h𝓐X (f⁻¹.[X]) (v₂)
+                    let u₁ := Iff.mp (hProp 𝓐 𝓑 f (f⁻¹.[X]) (v₂) (hiso)) u₀
+                    eq_subst (fun (t) => φ 𝓑 t) (f.[f⁻¹.[X]]) (X) (bijimg_f_finv f (setPO(𝓐)) (setPO(𝓑)) hfbij X hX) (u₁)
+
+            )
+            (
+              fun (h𝓑X) =>
+                fun (X) =>
+                  let v₀ := specification_set_subset (fun (b) => ∃ a ∈ X; (a . (f) . b)) (rng (f))
+                  let v₁ := rng_partial_function (f) (setPO(𝓐)) (setPO(𝓑)) (And.left hfunc)
+                  let v₂ := subset_trans (f.[X]) (rng (f)) (setPO(𝓑)) v₀ v₁
+                  fun (hX : X ⊆ setPO(𝓐)) =>
+                    Iff.mpr (hProp 𝓐 𝓑 f X hX hiso) (
+                      h𝓑X (f.[X]) (v₂)
+                    )
+            )
+      )
+
+
+
+theorem poiso_complatt : ∀ 𝓐 𝓑, (𝓐 P≃O 𝓑) → ((CompLatt 𝓐) ↔ (CompLatt 𝓑)) :=
+  fun (𝓐 𝓑 hPO) =>
+    let φ := fun (𝓐) => fun (X) => 𝓐 SuprExi X
+    let u₁ := poiso_subset_prop φ (poiso_supexi) 𝓐 𝓑 hPO
+    Iff.intro
+    (
+      fun (hcomp𝓐) =>
+        And.intro (And.left (And.right hPO)) (Iff.mp u₁ (And.right hcomp𝓐))
+    )
+    (
+      fun (hcomp𝓑) =>
+        And.intro (And.left hPO) (Iff.mpr u₁ (And.right hcomp𝓑))
+    )
 
 
 theorem poiso_linord : ∀ 𝓐 𝓑, (𝓐 P≃O 𝓑) → ((LinOrd 𝓐) ↔ (LinOrd 𝓑)) :=
@@ -9173,19 +9227,756 @@ theorem poiso_linord : ∀ 𝓐 𝓑, (𝓐 P≃O 𝓑) → ((LinOrd 𝓐) ↔ (
               fun (hφ₂φ₄) =>
                 And.intro (po𝓐) (Iff.mpr (u) (And.right hφ₂φ₄))
             )
-
-
-
       )
 
 
 
 
 
-theorem poiso_welord : ∀ 𝓐 𝓑, (𝓐 P≃O 𝓑) → ((WellOrd 𝓐) ↔ (WellOrd 𝓑)) := sorry
+theorem poiso_welord : ∀ 𝓐 𝓑, (𝓐 P≃O 𝓑) → ((WellOrd 𝓐) ↔ (WellOrd 𝓑)) :=
+  fun (𝓐 𝓑 hPO) =>
+    let φ := fun (𝓐) => fun (X) => (X ≠ ∅) → 𝓐 MinExi X
+
+    let u₀ := fun (𝓐 𝓑 f X) =>
+                fun (hX : X ⊆ setPO(𝓐)) =>
+                    fun (hf : f PO_ISO_PO 𝓐 To 𝓑) =>
+                      let hiso := And.right (And.right hf)
+                      let hbij := And.left hiso
+                      let hfunc := And.left hbij
+                      Iff.intro
+                      (
+                        fun (h𝓐 : (X ≠ ∅) → (𝓐 MinExi X)) =>
+                          fun (hfX : f.[X] ≠ ∅) =>
+                            Iff.mp (poiso_minexi 𝓐 𝓑 f X hX hf) (
+                              h𝓐 (Iff.mpr (set_non_empty_iff_non_empty X) (
+                                let u₁ := Iff.mp (set_non_empty_iff_non_empty (f.[X])) hfX
+                                Exists.elim u₁ (
+                                  fun (y) =>
+                                    fun (hy) =>
+                                      let u₂ := Iff.mp (image_prop f X y) hy
+                                      Exists.elim u₂ (
+                                        fun (x) =>
+                                          fun (hx) =>
+                                            Exists.intro x (And.left hx)
+                                      )
+                                )
+                              ))
+                            )
+                      )
+                      (
+                        fun (h𝓑 : (f.[X] ≠ ∅) → (𝓑 MinExi (f.[X]))) =>
+                          fun (hXemp : (X ≠ ∅)) =>
+                            Iff.mpr (poiso_minexi 𝓐 𝓑 f X hX hf) (
+                              h𝓑 (
+                                Iff.mpr (set_non_empty_iff_non_empty (f.[X])) (
+                                  let u₂ := Iff.mp (set_non_empty_iff_non_empty X) hXemp
+
+                                  Exists.elim u₂ (
+                                    fun (y) =>
+                                      fun (hy) =>
+                                        Exists.intro ((f⦅y⦆)) (
+                                          Iff.mpr (image_prop f X (f⦅y⦆)) (
+                                            Exists.intro y (
+                                              And.intro (hy) (
+                                                Iff.mpr (function_equal_value_prop f (setPO(𝓐)) (setPO(𝓑))
+                                                (hfunc) y (f⦅y⦆) (hX y hy)) (
+                                                  Eq.refl (f⦅y⦆)
+                                                )
+                                              )
+                                            )
+                                          )
+                                        )
+                                  )
+                                )
+                              )
+                            )
+                      )
+
+    let u₁ := poiso_subset_prop φ (u₀) 𝓐 𝓑 hPO
+    Iff.intro
+    (
+      fun (hWell𝓐) =>
+        And.intro (Iff.mp (poiso_linord 𝓐 𝓑 hPO) (And.left hWell𝓐)) (
+          Iff.mp (u₁) (And.right hWell𝓐)
+        )
+    )
+    (
+      fun (hWell𝓑) =>
+        And.intro (Iff.mpr (poiso_linord 𝓐 𝓑 hPO) (And.left hWell𝓑)) (
+          Iff.mpr (u₁) (And.right hWell𝓑)
+        )
+    )
 
 
-theorem poiso_inv : ∀ 𝓐, (𝓐 P≃O 𝓑) → ((inv_PO 𝓐) P≃O (inv_PO 𝓑)) := sorry
-theorem poiso_subs : ∀ 𝓐 𝓑 X, (X ⊆ setPO(𝓐)) → (f P≃O 𝓑) → (𝓐 SubsPO X) P≃O (𝓑 SubsPO (f.[X])) := sorry
-theorem poiso_inter : ∀ 𝓐 𝓑 𝓒 𝓓, (𝓐 P≃O 𝓑) → (𝓒 P≃O 𝓓) → ((𝓐 InterPO 𝓒) P≃O (𝓑 InterPO 𝓓)) := sorry
-theorem poiso_card : ∀ 𝓐 𝓑 𝓒 𝓓, (𝓐 P≃O 𝓑) → (𝓒 P≃O 𝓓) → ((𝓐 CartPO 𝓒) P≃O (𝓑 CartPO 𝓓)) := sorry
+theorem poiso_inv : ∀ 𝓐 𝓑, (𝓐 P≃O 𝓑) → ((inv_PO 𝓐) P≃O (inv_PO 𝓑)) :=
+  fun (𝓐 𝓑 hPO) =>
+    Exists.elim (And.right (And.right (hPO))) (
+      fun (f) =>
+        fun (hf) =>
+          let u₀ := And.left hf
+          And.intro (inv_is_PO 𝓐 (And.left hPO)) (And.intro (
+            inv_is_PO 𝓑 (And.left (And.right hPO))
+          ) (
+            let u₁ := setPO_is_setPO setPO(𝓐) ≻(𝓐) ≽(𝓐)
+            let u₂ := setPO_is_setPO setPO(𝓑) ≻(𝓑) ≽(𝓑)
+            Exists.intro f (
+              And.intro (
+                eq_subst (fun (t) => (f Bij (setPO(inv_PO 𝓐)) To t)) (setPO(𝓑)) (setPO(inv_PO 𝓑)) (Eq.symm u₂) (
+                  eq_subst (fun (s) => (f Bij s To setPO(𝓑))) (setPO(𝓐)) (setPO(inv_PO 𝓐)) (Eq.symm u₁) (
+                    u₀
+                  )
+                )
+              ) (
+                fun (x hx y hy) =>
+                    let hx₁ := eq_subst (fun (t) => x ∈ t) (setPO(inv_PO 𝓐)) (setPO(𝓐)) (u₁) hx
+                    let hy₁ := eq_subst (fun (t) => y ∈ t) (setPO(inv_PO 𝓐)) (setPO(𝓐)) (u₁) hy
+                    let u₃ := And.right hf y hy₁ x hx₁
+                    let u₄ := po_lesseq_moreeq 𝓐 (And.left hPO) y x
+                    let u₅ := po_lesseq_moreeq 𝓑 (And.left (And.right hPO)) (f⦅y⦆) (f⦅x⦆)
+                    let v₀ := lesseqPO_is_lesseqPO setPO(𝓐) ≻(𝓐) ≽(𝓐)
+                    let v₀₀ := lesseqPO_is_lesseqPO setPO(𝓑) ≻(𝓑) ≽(𝓑)
+                    Iff.intro
+                    (
+                      fun (hxy) =>
+
+                        let v₁ := eq_subst (fun (t) => (x, y) ∈ t) (≼(inv_PO 𝓐)) (≽(𝓐)) (v₀) (hxy)
+                        let v₂ := Iff.mpr u₄ v₁
+                        let v₃ := Iff.mp u₃ v₂
+                        let v₄ := Iff.mp u₅ v₃
+                        eq_subst (fun (t) => ((f⦅x⦆), (f⦅y⦆)) ∈ t) (≽(𝓑)) (≼(inv_PO 𝓑)) (Eq.symm v₀₀) (v₄)
+                    )
+                    (
+                      fun (hfxy) =>
+                        let v₁ := eq_subst (fun (t) => ((f⦅x⦆), (f⦅y⦆)) ∈ t) (≼(inv_PO 𝓑)) (≽(𝓑)) (v₀₀) (hfxy)
+                        let v₂ := Iff.mpr u₅ v₁
+                        let v₃ := Iff.mpr u₃ v₂
+                        let v₄ := Iff.mp u₄ v₃
+                        eq_subst (fun (t) => ((x), (y)) ∈ t) (≽(𝓐)) (≼(inv_PO 𝓐)) (Eq.symm v₀) (v₄)
+                    )
+              )
+            )
+          ))
+    )
+
+
+theorem poiso_subs : ∀ 𝓐 𝓑 f X, (X ≠ ∅) → (X ⊆ setPO(𝓐)) → (f PO_ISO_PO 𝓐 To 𝓑) → ((𝓐 SubsPO X) P≃O (𝓑 SubsPO (f.[X]))) :=
+  fun (𝓐 𝓑 f X hempX hX) =>
+    fun (hf : (f PO_ISO_PO 𝓐 To 𝓑)) =>
+      let hiso := And.right (And.right hf)
+      let hbij := And.left hiso
+      let hfunc := And.left hbij
+      let A := setPO(𝓐)
+      let B := setPO(𝓑)
+      let u₁ := Iff.mp (set_non_empty_iff_non_empty X) hempX
+      Exists.elim u₁ (
+        fun (x) =>
+          fun (hx) =>
+            let u₂ := Iff.mpr (image_prop f X (f⦅x⦆)) (
+              Exists.intro x (And.intro (hx) (function_value_pick_property f A B x (hX x hx) (And.left hbij)))
+            )
+
+            let u₃ := Iff.mpr (set_non_empty_iff_non_empty (f.[X])) (
+              Exists.intro (f⦅x⦆) (u₂)
+            )
+
+            let v₀ := specification_set_subset (fun (b) => ∃ a ∈ X; (a . (f) . b)) (rng (f))
+            let v₁ := rng_partial_function (f) (setPO(𝓐)) (setPO(𝓑)) (And.left hfunc)
+            let v₂ := subset_trans (f.[X]) (rng (f)) (setPO(𝓑)) v₀ v₁
+            let v₃ := setPO_is_setPO X (≺(𝓐) spec X) (≼(𝓐) spec X)
+            let v₄ := setPO_is_setPO (f.[X]) (≺(𝓑) spec (f.[X])) (≼(𝓑) spec (f.[X]))
+            let v₄₁ := lesseqPO_is_lesseqPO X (≺(𝓐) spec X) (≼(𝓐) spec X)
+            let v₄₂ := lesseqPO_is_lesseqPO (f.[X]) (≺(𝓑) spec (f.[X])) (≼(𝓑) spec (f.[X]))
+
+            And.intro (sub_is_PO 𝓐 X hempX (And.left hf) hX) (
+              And.intro (sub_is_PO 𝓑 (f.[X]) u₃ (And.left (And.right hf)) (v₂)) (
+                Exists.intro (f ⨡ X) (
+                  And.intro (
+
+                    eq_subst (fun (t) => (f ⨡ X) Bij t To setPO(𝓑 SubsPO (f.[X]))) (X) (setPO(𝓐 SubsPO X)) (Eq.symm v₃) (
+                      eq_subst (fun (t₂) => (f ⨡ X) Bij X To t₂) (f.[X]) (setPO(𝓑 SubsPO (f.[X]))) (Eq.symm v₄) (
+                        equinum_image_f A B X f hX (And.intro (hfunc) (And.left (And.right hbij)))
+                      )
+                    )
+
+                  ) (
+                    fun (x) =>
+                      fun (hx) =>
+                        fun (y) =>
+                          fun (hy) =>
+                            let hx₁ := eq_subst (fun (t) => x ∈ t) (setPO(𝓐 SubsPO X)) X (v₃) (hx)
+                            let hy₁ := eq_subst (fun (t) => y ∈ t) (setPO(𝓐 SubsPO X)) (X) (v₃) (hy)
+                            let hx₂ := hX x hx₁
+                            let hy₂ := hX y hy₁
+
+                            Iff.intro
+                            (
+                              fun (hxy) =>
+                                let v₅ := eq_subst (fun (t) => (x, y) ∈ t) (≼(𝓐 SubsPO X)) (≼(𝓐) spec X) (v₄₁) (hxy)
+                                let v₆ := interset2sets_subset_prop (≼(𝓐)) (X × X)
+                                let v₇ := And.left v₆ (x, y) v₅
+                                let v₈ := Iff.mp (And.right hiso x hx₂ y hy₂) v₇
+                                let v₉ := fun_restriction_val A B X f hX hfunc x hx₁
+                                let v₁₀ := fun_restriction_val A B X f hX hfunc y hy₁
+                                let v₁₁ := eq_subst (fun (t) => (t, ((f ⨡ X)⦅y⦆)) ∈ (≼(𝓑))) (f⦅x⦆) ((f ⨡ X)⦅x⦆) (v₉) (
+                                  eq_subst (fun (t) => ((f⦅x⦆), t) ∈ (≼(𝓑)) ) (f⦅y⦆) ((f ⨡ X)⦅y⦆) (v₁₀) (v₈)
+                                )
+                                let m := (f ⨡ X)⦅x⦆
+                                let n := (f ⨡ X)⦅y⦆
+
+                                let himg₁ := Iff.mpr (image_prop f X (f⦅x⦆)) (
+                                  Exists.intro x (And.intro (hx₁) (function_value_pick_property f A B x hx₂ hfunc))
+                                )
+
+                                let himg₂ := Iff.mpr (image_prop f X (f⦅y⦆)) (
+                                  Exists.intro y (And.intro (hy₁) (function_value_pick_property f A B y hy₂ hfunc))
+                                )
+
+
+                                eq_subst (fun (t) => (m, n) ∈ t) (≼(𝓑) spec (f.[X])) (≼(𝓑 SubsPO (f.[X]))) (Eq.symm v₄₂) (
+                                  Iff.mpr (intersect_2sets_prop (≼(𝓑)) (f.[X] × f.[X]) (m, n)) (
+                                    And.intro (v₁₁) (
+                                      Iff.mpr (cartesian_product_pair_prop (f.[X]) (f.[X]) m n) (
+                                        And.intro (
+                                          eq_subst (fun (t) => (t) ∈ (f.[X])) (f⦅x⦆) m (v₉) (
+                                            himg₁
+                                          )
+                                        ) (eq_subst (fun (t) => (t) ∈ (f.[X])) (f⦅y⦆) n (v₁₀) (
+                                            himg₂
+                                          ))
+                                      )
+                                    )
+                                  )
+                                )
+                            )
+                            (
+                              fun (hfxy) =>
+                                let m := (f ⨡ X)⦅x⦆
+                                let n := (f ⨡ X)⦅y⦆
+                                let s₁ := eq_subst (fun (t) => (m, n) ∈ t) (≼(𝓑 SubsPO (f.[X]))) (≼(𝓑) spec (f.[X])) (v₄₂) (hfxy)
+                                let s₂ := Iff.mp (intersect_2sets_prop (≼(𝓑)) (f.[X] × f.[X]) (m, n)) s₁
+                                let s₃ := And.left s₂
+                                let s₅ := fun_restriction_val A B X f hX hfunc x hx₁
+                                let s₆ := fun_restriction_val A B X f hX hfunc y hy₁
+                                let s₇ := eq_subst (fun (t) => (t, (f⦅y⦆)) ∈ ≼(𝓑)) ((f ⨡ X)⦅x⦆) (f⦅x⦆) (Eq.symm s₅) (
+                                  eq_subst (fun (t) => (((f ⨡ X)⦅x⦆), t) ∈ ≼(𝓑)) ((f ⨡ X)⦅y⦆) (f⦅y⦆) (Eq.symm s₆) (
+                                    s₃
+                                  )
+                                )
+                                let s₈ := Iff.mpr (And.right hiso x hx₂ y hy₂) s₇
+                                let s₉ := Iff.mpr (intersect_2sets_prop (≼(𝓐)) (X × X) (x, y)) (
+                                  And.intro (s₈) (
+                                    Iff.mpr (cartesian_product_pair_prop X X x y) (
+                                      And.intro (hx₁) (hy₁)
+                                    )
+                                  )
+                                )
+                                eq_subst (fun (t) => (x, y) ∈ t) (≼(𝓐) spec X) (≼(𝓐 SubsPO X)) (Eq.symm (v₄₁)) (s₉)
+                            )
+                  )
+                )
+              )
+            )
+      )
+
+
+
+
+theorem poiso_inter : ∀ 𝓐 𝓑 𝓒 𝓓 f, (setPO(𝓐) = setPO(𝓒)) →
+(setPO(𝓑) = setPO(𝓓)) → (f PO_ISO_PO 𝓐 To 𝓑) → (f PO_ISO_PO 𝓒 To 𝓓) → (f PO_ISO_PO (𝓐 InterPO 𝓒) To (𝓑 InterPO 𝓓)) :=
+  fun (𝓐 𝓑 𝓒 𝓓 f heq₁ heq₂ h𝓐𝓑 h𝓒𝓓) =>
+          let u₁ := setPO_is_setPO (setPO(𝓐)) (≺(𝓐) ∩ ≺(𝓒)) (≼(𝓐) ∩ ≼(𝓒))
+          let u₂ := setPO_is_setPO (setPO(𝓑)) (≺(𝓑) ∩ ≺(𝓓)) (≼(𝓑) ∩ ≼(𝓓))
+          let u₃ := lesseqPO_is_lesseqPO (setPO(𝓐)) (≺(𝓐) ∩ ≺(𝓒)) (≼(𝓐) ∩ ≼(𝓒))
+          let u₄ := lesseqPO_is_lesseqPO (setPO(𝓑)) (≺(𝓑) ∩ ≺(𝓓)) (≼(𝓑) ∩ ≼(𝓓))
+          let u₀ := And.right (And.right (h𝓐𝓑))
+          let u₀₁:= And.right (And.right h𝓒𝓓)
+          And.intro (inter_is_PO_PO 𝓐 𝓒 (And.left h𝓐𝓑) (And.left h𝓒𝓓) heq₁) (
+            And.intro (inter_is_PO_PO 𝓑 𝓓 (And.left (And.right h𝓐𝓑)) (And.left (And.right h𝓒𝓓)) heq₂) (
+              And.intro (
+
+                eq_subst (fun (t) => f Bij t To setPO(𝓑 InterPO 𝓓)) (setPO(𝓐)) (setPO(𝓐 InterPO 𝓒)) (Eq.symm u₁) (
+                  eq_subst (fun (s) => f Bij (setPO(𝓐)) To s) (setPO(𝓑)) (setPO(𝓑 InterPO 𝓓)) (Eq.symm u₂) (
+                    And.left u₀
+                  )
+                )
+
+              ) (
+                fun (x hx y hy) =>
+                  let hx₁ := eq_subst (fun (t) => x ∈ t) (setPO(𝓐 InterPO 𝓒)) (setPO(𝓐)) (u₁) (hx)
+                  let hx₂ := eq_subst (fun (t) => x ∈ t) (setPO(𝓐)) (setPO(𝓒)) (heq₁) (hx₁)
+                  let hy₁ := eq_subst (fun (t) => y ∈ t) (setPO(𝓐 InterPO 𝓒)) (setPO(𝓐)) (u₁) (hy)
+                  let hy₂ := eq_subst (fun (t) => y ∈ t) (setPO(𝓐)) (setPO(𝓒)) (heq₁) (hy₁)
+                  Iff.intro
+                  (
+                    fun (hxy) =>
+                      let u₅ := eq_subst (fun (t) => (x, y) ∈ t) (≼(𝓐 InterPO 𝓒)) (≼(𝓐) ∩ (≼(𝓒))) (u₃) hxy
+                      let u₆ := Iff.mp (intersect_2sets_prop (≼(𝓐)) (≼(𝓒)) (x, y)) u₅
+                      let u₇ := Iff.mp (And.right u₀ x hx₁ y hy₁) (And.left u₆)
+                      let u₈ := Iff.mp (And.right u₀₁ x hx₂ y hy₂) (And.right u₆)
+
+                      eq_subst (fun (t) => ((f⦅x⦆), (f⦅y⦆)) ∈ t) (≼(𝓑) ∩ ≼(𝓓)) (≼(𝓑 InterPO 𝓓)) (Eq.symm u₄) (
+                        Iff.mpr (intersect_2sets_prop (≼(𝓑)) (≼(𝓓)) ((f⦅x⦆), (f⦅y⦆)) ) (
+                          And.intro (u₇) (u₈)
+                        )
+                      )
+                  )
+                  (
+                    fun (hfxy) =>
+                      let u₅ := eq_subst (fun (t) => ((f⦅x⦆), (f⦅y⦆)) ∈ t) (≼(𝓑 InterPO 𝓓)) (≼(𝓑) ∩ ≼(𝓓)) (u₄) hfxy
+                      let u₆ := Iff.mp (intersect_2sets_prop (≼(𝓑)) (≼(𝓓)) ((f⦅x⦆), (f⦅y⦆))) u₅
+                      let u₇ := Iff.mpr (And.right u₀ x hx₁ y hy₁) (And.left u₆)
+                      let u₈ := Iff.mpr (And.right u₀₁ x hx₂ y hy₂) (And.right u₆)
+
+                      eq_subst (fun (t) => (x, y) ∈ t) (≼(𝓐) ∩ (≼(𝓒))) (≼(𝓐 InterPO 𝓒)) (Eq.symm u₃) (
+                        Iff.mpr (intersect_2sets_prop (≼(𝓐)) (≼(𝓒)) (x, y)) (
+                          And.intro (u₇) (u₈)
+                        )
+                      )
+                  )
+              )
+            )
+          )
+
+
+
+
+theorem poiso_cart : ∀ 𝓐 𝓑 𝓒 𝓓, (𝓐 P≃O 𝓑) → (𝓒 P≃O 𝓓) → ((𝓐 CartPO 𝓒) P≃O (𝓑 CartPO 𝓓)) :=
+  fun (𝓐 𝓑 𝓒 𝓓 h𝓐𝓑 h𝓒𝓓) =>
+    let hpo𝓐𝓑 := And.right (And.right h𝓐𝓑)
+    let h𝓐 := And.left h𝓐𝓑
+    let h𝓑 := And.left (And.right h𝓐𝓑)
+    let hpo𝓒𝓓 := And.right (And.right h𝓒𝓓)
+    let h𝓒 := And.left h𝓒𝓓
+    let h𝓓 := And.left (And.right h𝓒𝓓)
+    let A := setPO(𝓐)
+    let B := setPO(𝓑)
+    let C := setPO(𝓒)
+    let D := setPO(𝓓)
+    let u₁ := setPO_is_setPO (A × C) (le_cart 𝓐 𝓒) (leq_cart 𝓐 𝓒)
+    let u₂ := setPO_is_setPO (B × D) (le_cart 𝓑 𝓓) (leq_cart 𝓑 𝓓)
+    let u₁₁ := lesseqPO_is_lesseqPO (A × C) (le_cart 𝓐 𝓒) (leq_cart 𝓐 𝓒)
+    let u₂₁ := lesseqPO_is_lesseqPO (B × D) (le_cart 𝓑 𝓓) (leq_cart 𝓑 𝓓)
+
+    Exists.elim hpo𝓐𝓑 (
+      fun (f) =>
+        fun (hf) =>
+          Exists.elim hpo𝓒𝓓 (
+            fun (g) =>
+              fun (hg) =>
+                And.intro (cart_PO_PO 𝓐 𝓒 h𝓐 h𝓒) (And.intro (
+                  cart_PO_PO 𝓑 𝓓 h𝓑 h𝓓
+                ) (
+                  let hf₁ := And.left hf
+                  let hf₂ := And.left hf₁
+                  let hf₃ := And.intro hf₂ (And.left (And.right hf₁))
+                  let hg₁ := And.left hg
+                  let hg₂ := And.left hg₁
+                  let hg₃ := And.intro hg₂ (And.left (And.right hg₁))
+                  let hf₄ := And.right hf
+                  let hg₄ := And.right hg
+                  let hfinv := bijection_inv_mp f A B hf₁
+                  let hginv := bijection_inv_mp g C D hg₁
+                  let X := A × C
+                  let Y := B × D
+                  let P := fun (pr) => (f⦅π₁ pr⦆, g⦅π₂ pr⦆)
+                  let h := lam_fun (A × C) (B × D) P
+                  let func_prop_all := lam_then_fun_prop (P) X Y (
+                      fun (elem) => fun (h₂ : elem ∈ X) =>
+                        let h₅ := fst_coor_set A C elem h₂
+                        let h₇ := val_in_B f A B hf₂ (π₁ elem) (h₅)
+                        let h₀ := snd_coor_set A C elem h₂
+                        let h₀₀ := val_in_B g C D hg₂ (π₂ elem) (h₀)
+                        Iff.mpr (cartesian_product_pair_prop B D (f⦅π₁ elem⦆) (g⦅π₂ elem⦆)) (
+                          And.intro (h₇) (h₀₀)
+                        )
+                  )
+                  let func_prop := And.left func_prop_all
+                  let value_prop := And.right func_prop_all
+                  let inj_prop := Iff.mpr (func_inj_prop X Y h func_prop) (
+                    fun (x hx y hy) =>
+                      fun (hxhy) =>
+                        let u₃ := value_prop x hx
+                        let u₄ := value_prop y hy
+                        let u₅ := Eq.trans (Eq.symm u₃) (hxhy)
+                        let u₆ := Eq.trans (u₅) (u₄)
+                        let u₇ := Iff.mp (ordered_pair_set_prop (f⦅π₁ x⦆) (g⦅π₂ x⦆) (f⦅π₁ y⦆) (g⦅π₂ y⦆)) u₆
+                        let u₇₀ := fst_coor_set A C x hx
+                        let u₇₁ := fst_coor_set A C y hy
+                        let u₇₂ := snd_coor_set A C x hx
+                        let u₇₃ := snd_coor_set A C y hy
+                        let u₈ := Iff.mp (func_inj_prop A B f hf₂) (hf₃) (π₁ x) u₇₀ (π₁ y) u₇₁ (And.left u₇)
+                        let u₉ := Iff.mp (func_inj_prop C D g hg₂) (hg₃) (π₂ x) u₇₂ (π₂ y) (u₇₃) (And.right u₇)
+                        equal_fst_snd A C x y hx hy u₈ u₉
+                  )
+                  let injv_prop := And.right inj_prop
+                  let surj_prop := Iff.mpr (func_surj_prop X Y h func_prop) (
+                    fun (s hs) =>
+                      let lelem := ((f⁻¹)⦅π₁ s⦆)
+                      let relem := ((g⁻¹)⦅π₂ s⦆)
+                      let elem := ((((f⁻¹)⦅π₁ s⦆)), ((g⁻¹)⦅π₂ s⦆))
+
+                      Exists.intro elem (
+                        let u₃ := fst_coor_set B D s hs
+                        let u₄ := val_in_B (f⁻¹) B A (And.left hfinv) (π₁ s) u₃
+                        let u₅ := snd_coor_set B D s hs
+                        let u₆ := val_in_B (g⁻¹) D C (And.left hginv) (π₂ s) u₅
+                        let u₇ := Iff.mpr (cartesian_product_pair_prop A C ((f⁻¹)⦅π₁ s⦆) ((g⁻¹)⦅π₂ s⦆)) (
+                          And.intro (u₄) (u₆)
+                        )
+                        And.intro (u₇) (
+
+                          let u₈ := value_prop elem u₇
+                          Eq.trans (
+                            let u₉ := coordinates_fst_coor lelem relem
+                            let u₁₀ := eq_subst (fun (t) => (f⦅π₁ elem⦆) = (f⦅t⦆)) (π₁ elem) (lelem) (u₉) (Eq.refl (f⦅π₁ elem⦆))
+                            let u₁₁ := bij_f_finv f A B hf₁ (π₁ s) u₃
+                            let u₁₂ := Eq.trans u₁₀ u₁₁
+                            let u₁₃ := coordinates_snd_coor lelem relem
+                            let u₁₄ := eq_subst (fun (t) => (g⦅π₂ elem⦆) = (g⦅t⦆)) (π₂ elem) (relem) (u₁₃) (Eq.refl (g⦅π₂ elem⦆))
+                            let u₁₅ := bij_f_finv g C D hg₁ (π₂ s) u₅
+                            let u₁₆ := Eq.trans u₁₄ u₁₅
+                            let u₁₇ := Iff.mpr (ordered_pair_set_prop (f⦅π₁ elem⦆) (g⦅π₂ elem⦆) (π₁ s) (π₂ s)) (
+                              And.intro (u₁₂) (u₁₆)
+                            )
+                            let u₁₈ := fst_snd_then_unique B D s hs
+                            Eq.trans (u₁₈) (Eq.symm u₁₇)
+
+                          ) (Eq.symm u₈)
+                        )
+                      )
+
+                  )
+                  let surjv_prop := And.right surj_prop
+                  Exists.intro h (
+                    And.intro (
+                      eq_subst (fun (t) => h Bij t To (setPO(𝓑 CartPO 𝓓))) (A × C) (setPO(𝓐 CartPO 𝓒)) (Eq.symm u₁) (
+                        eq_subst (fun (t) => h Bij (A × C) To t) (B × D) (setPO(𝓑 CartPO 𝓓)) (Eq.symm u₂) (
+                          And.intro (func_prop) (And.intro (injv_prop) (surjv_prop))
+                        )
+                      )
+                    ) (
+
+
+                      fun (x hx y hy) =>
+
+                        let hx₁ := eq_subst (fun (t) => x ∈ t) (setPO(𝓐 CartPO 𝓒)) (A × C) (u₁) hx
+                        let hx₁₁ := fst_coor_set A C x hx₁
+                        let hx₁₂ := snd_coor_set A C x hx₁
+                        let hy₁ := eq_subst (fun (t) => y ∈ t) (setPO(𝓐 CartPO 𝓒)) (A × C) (u₁) hy
+                        let hy₁₁ := fst_coor_set A C y hy₁
+                        let hy₁₂ := snd_coor_set A C y hy₁
+                        let hhx := val_in_B h X Y func_prop x hx₁
+                        let hhy := val_in_B h X Y func_prop y hy₁
+                        let v₃ : (π₁ (P x)) = (f⦅π₁ x⦆) := coordinates_fst_coor (f⦅π₁ x⦆) (g⦅π₂ x⦆)
+                        let v₄ := value_prop x hx₁
+                        let v₅ := eq_subst (fun (t) => (π₁ t) = (f⦅π₁ x⦆)) (P x) (h⦅x⦆) (Eq.symm v₄) v₃
+
+                        let v₆ : (π₁ (P y)) = (f⦅π₁ y⦆) := coordinates_fst_coor (f⦅π₁ y⦆) (g⦅π₂ y⦆)
+                        let v₇ := value_prop y hy₁
+                        let v₈ := eq_subst (fun (t) => (π₁ t) = (f⦅π₁ y⦆)) (P y) (h⦅y⦆) (Eq.symm v₇) v₆
+
+                        let v₃₁ : (π₂ (P x)) = (g⦅π₂ x⦆) := coordinates_snd_coor (f⦅π₁ x⦆) (g⦅π₂ x⦆)
+                        let v₄₁ := value_prop x hx₁
+                        let v₅₁ := eq_subst (fun (t) => (π₂ t) = (g⦅π₂ x⦆)) (P x) (h⦅x⦆) (Eq.symm v₄₁) v₃₁
+
+                        let v₆₁ : (π₂ (P y)) = (g⦅π₂ y⦆) := coordinates_snd_coor (f⦅π₁ y⦆) (g⦅π₂ y⦆)
+                        let v₇₁ := value_prop y hy₁
+                        let v₈₁ := eq_subst (fun (t) => (π₂ t) = (g⦅π₂ y⦆)) (P y) (h⦅y⦆) (Eq.symm v₇₁) v₆₁
+
+                        Iff.intro
+                        (
+                          fun (hxy) =>
+                            let v₀₀ := eq_subst (fun (t) => (x, y) ∈ t) (≼(𝓐 CartPO 𝓒)) (leq_cart 𝓐 𝓒) (u₁₁) (hxy)
+                            let v₀ := Iff.mp (leq_cart_prop 𝓐 𝓒 x hx₁ y hy₁) v₀₀
+                            let v₁ := Iff.mp (hf₄ (π₁ x) (hx₁₁) (π₁ y) (hy₁₁)) (And.left v₀)
+                            let v₂ := Iff.mp (hg₄ (π₂ x) (hx₁₂) (π₂ y) (hy₁₂)) (And.right v₀)
+
+                            let v₉ := eq_subst (fun (t) => (t, (π₁ (h⦅y⦆))) ∈ (≼(𝓑))) (f⦅π₁ x⦆) (π₁ (h⦅x⦆)) (Eq.symm v₅) (
+                              eq_subst (fun (t) => ((f⦅π₁ x⦆), t) ∈ (≼(𝓑))) (f⦅π₁ y⦆) (π₁ (h⦅y⦆)) (Eq.symm v₈) (v₁)
+                            )
+                            let v₉₁ := eq_subst (fun (t) => (t, (π₂ (h⦅y⦆))) ∈ (≼(𝓓))) (g⦅π₂ x⦆) (π₂ (h⦅x⦆)) (Eq.symm v₅₁) (
+                              eq_subst (fun (t) => ((g⦅π₂ x⦆), t) ∈ (≼(𝓓))) (g⦅π₂ y⦆) (π₂ (h⦅y⦆)) (Eq.symm v₈₁) (v₂)
+                            )
+                            let v := Iff.mpr (leq_cart_prop 𝓑 𝓓 (h⦅x⦆) hhx (h⦅y⦆) hhy) (
+                              And.intro (v₉) (v₉₁)
+                            )
+
+                            eq_subst (fun (t) => ((h⦅x⦆), (h⦅y⦆)) ∈ t) (leq_cart 𝓑 𝓓) (≼(𝓑 CartPO 𝓓)) (Eq.symm u₂₁) (v)
+                        )
+                        (
+                          fun (hfxy) =>
+                            let v₀₀ := eq_subst (fun (t) => ((h⦅x⦆), (h⦅y⦆)) ∈ t) (≼(𝓑 CartPO 𝓓)) (leq_cart 𝓑 𝓓) (u₂₁) (hfxy)
+                            let v₀ := Iff.mp (leq_cart_prop 𝓑 𝓓 (h⦅x⦆) hhx (h⦅y⦆) hhy) v₀₀
+
+                            let v₉ := eq_subst (fun (t) => (t, (f⦅π₁ y⦆)) ∈ (≼(𝓑))) (π₁ (h⦅x⦆)) (f⦅π₁ x⦆) (v₅) (
+                              eq_subst (fun (t) => ((π₁ (h⦅x⦆)), t) ∈ (≼(𝓑))) (π₁ (h⦅y⦆)) (f⦅π₁ y⦆) v₈ (
+                                And.left v₀
+                              )
+                            )
+
+                            let v₉₁ := eq_subst (fun (t) => (t, (g⦅π₂ y⦆)) ∈ (≼(𝓓))) (π₂ (h⦅x⦆)) (g⦅π₂ x⦆) (v₅₁) (
+                              eq_subst (fun (t) => ((π₂ (h⦅x⦆)), t) ∈ (≼(𝓓))) (π₂ (h⦅y⦆)) (g⦅π₂ y⦆) v₈₁ (
+                                And.right v₀
+                              )
+                            )
+
+                            let v₂ := Iff.mpr (hg₄ (π₂ x) (hx₁₂) (π₂ y) (hy₁₂)) v₉₁
+                            let v₁ := Iff.mpr (hf₄ (π₁ x) (hx₁₁) (π₁ y) (hy₁₁)) v₉
+                            let v₃ := Iff.mpr (leq_cart_prop 𝓐 𝓒 x hx₁ y hy₁) (And.intro (v₁) (v₂))
+
+                            eq_subst (fun (t) => (x, y) ∈ t) (leq_cart 𝓐 𝓒) (≼(𝓐 CartPO 𝓒)) (Eq.symm u₁₁) (v₃)
+                        )
+
+                    )
+                  )
+                ))
+          )
+    )
+
+noncomputable def induced_R₂ (𝓐 f: Set) := {s ∈ (rng f) × (rng f) | ∃ x y ∈ setPO(𝓐); (x . (≼(𝓐)) . y) ∧ s = (f⦅x⦆, f⦅y⦆)}
+
+theorem bij_rng : ∀ f A B, (f Inj A To B) → (f Bij A To (rng f)) :=
+  fun (f A B) =>
+    fun (hinf) =>
+      let hfrngf := function_rng_def f A B (And.left hinf)
+      And.intro (hfrngf) (
+        And.intro (And.right hinf) (
+          fun (y) =>
+            fun (hy) =>
+              Iff.mp (rng_prop f y) hy
+        )
+      )
+
+
+theorem induced_crit₀ : ∀ 𝓐 f, (f Bij (setPO(𝓐)) To (rng f)) → ∀ x y ∈ (setPO(𝓐)); (x . (≼(𝓐)) . y) ↔ ((f⦅x⦆) . (induced_R₂ 𝓐 f) . (f⦅y⦆)) :=
+  fun (𝓐 f hf) =>
+    fun (x hx y hy) =>
+      let P := fun (s) => ∃ x y ∈ setPO(𝓐); (x . (≼(𝓐)) . y) ∧ s = (f⦅x⦆, f⦅y⦆)
+      let rn := rng f
+      let B := (rn) × (rn)
+      let fxset := val_in_B f (setPO(𝓐)) rn (And.left hf) x hx
+      let fyset := val_in_B f (setPO(𝓐)) rn (And.left hf) y hy
+      Iff.intro
+      (
+        fun (hxy) =>
+          Iff.mpr (spec_is_spec P B ((f⦅x⦆), (f⦅y⦆))) (
+            And.intro (
+
+              Iff.mpr (cartesian_product_pair_prop rn rn (f⦅x⦆) (f⦅y⦆)) (
+                And.intro (fxset) (fyset)
+              )
+
+            ) (Exists.intro x (And.intro (hx) (Exists.intro y (And.intro (hy) (
+              And.intro (hxy) (Eq.refl ((f⦅x⦆), (f⦅y⦆)))
+            )))))
+          )
+      )
+      (
+        fun (hfxy) =>
+          let u₁ := And.right (Iff.mp (spec_is_spec P B ((f⦅x⦆), (f⦅y⦆))) hfxy)
+          Exists.elim u₁ (
+            fun (a) =>
+              fun (ha) =>
+                Exists.elim (And.right ha) (
+                  fun (b) =>
+                    fun (hb) =>
+                      let u₂ := And.right hb
+                      let u₃ := And.right u₂
+                      let u₄ := Iff.mp (ordered_pair_set_prop (f⦅x⦆) (f⦅y⦆) (f⦅a⦆) (f⦅b⦆)) u₃
+                      let u₅ := And.intro (And.left hf) (And.left (And.right hf))
+                      let u₆ := Iff.mp (func_inj_prop (setPO(𝓐)) (rng f) f (And.left u₅)) u₅ x hx a (And.left ha) (And.left u₄)
+                      let u₇ := Iff.mp (func_inj_prop (setPO(𝓐)) (rng f) f (And.left u₅)) u₅ y hy b (And.left hb) (And.right u₄)
+                      let u₈ := eq_subst (fun (t) => (t, b) ∈ (≼(𝓐))) a x (Eq.symm u₆) (And.left u₂)
+                      eq_subst (fun (t) => (x, t) ∈ (≼(𝓐))) b y (Eq.symm u₇) (u₈)
+                )
+          )
+
+
+      )
+
+
+
+theorem induced_crit: ∀ 𝓐 f, (f Bij (setPO(𝓐)) To (rng f)) →  ∀ x y ∈ rng f; (x . (induced_R₂ 𝓐 f) . y) ↔ (((f⁻¹⦅x⦆) . (≼(𝓐)) . (f⁻¹⦅y⦆))) :=
+fun (𝓐 f hf) =>
+  fun (x hx y hy) =>
+    let P := fun (s) => ∃ x y ∈ setPO(𝓐); (x . (≼(𝓐)) . y) ∧ s = (f⦅x⦆, f⦅y⦆)
+    let rn := rng f
+    let B := (rn) × (rn)
+    let finvbij := bijection_inv_mp f (setPO(𝓐)) (rng f) hf
+    let finvfunc := And.left finvbij
+    Iff.intro
+    (
+      fun (hxy) =>
+        let u₁ := Iff.mp (spec_is_spec P B (x, y)) hxy
+        Exists.elim (And.right u₁) (
+          fun (a) =>
+            fun (ha) =>
+              Exists.elim (And.right ha) (
+                fun (b) =>
+                  fun (hb) =>
+                    let u₂ := And.right hb
+                    let u₃ := And.right u₂
+                    let u₄ := Iff.mp (ordered_pair_set_prop x y (f⦅a⦆) (f⦅b⦆)) u₃
+                    let u₅ := And.left u₄
+                    let u₆ := eq_subst (fun (t) => (f⁻¹⦅x⦆) = (f⁻¹⦅t⦆)) x (f⦅a⦆) (u₅) (Eq.refl (f⁻¹⦅x⦆))
+                    let u₇ := bij_finv_f f (setPO(𝓐)) rn hf a (And.left ha)
+                    let u₈ := Eq.trans u₆ u₇
+                    let u₉ := And.right u₄
+                    let u₁₀ := eq_subst (fun (t) => (f⁻¹⦅y⦆) = (f⁻¹⦅t⦆)) y (f⦅b⦆) (u₉) (Eq.refl (f⁻¹⦅y⦆))
+                    let u₁₁ := bij_finv_f f (setPO(𝓐)) rn hf b (And.left hb)
+                    let u₁₂ := Eq.trans u₁₀ u₁₁
+
+                    let u₁₃ := And.left u₂
+                    let u₁₄ := eq_subst (fun (t) => (t, b) ∈ (≼(𝓐))) (a) (f⁻¹⦅x⦆) (Eq.symm u₈) (u₁₃)
+                    eq_subst (fun (t) => ((f⁻¹⦅x⦆), t) ∈ (≼(𝓐))) (b) (f⁻¹⦅y⦆) (Eq.symm u₁₂) (u₁₄)
+              )
+        )
+
+    )
+    (
+      fun (hfxy) =>
+        let u₁ := Iff.mpr (cartesian_product_pair_prop rn rn x y) (And.intro (hx) (hy))
+        let u₂ := val_in_B (f⁻¹) (rn) (setPO(𝓐)) finvfunc x hx
+        let u₃ := val_in_B (f⁻¹) (rn) (setPO(𝓐)) finvfunc y hy
+
+        Iff.mpr (spec_is_spec P B (x, y)) (
+
+          And.intro (u₁) (
+            Exists.intro (f⁻¹⦅x⦆) (
+              And.intro (u₂) (Exists.intro (f⁻¹⦅y⦆) (
+
+                And.intro (u₃) (
+                  And.intro (hfxy) (
+                    Iff.mpr (ordered_pair_set_prop x y (f⦅f⁻¹⦅x⦆⦆) (f⦅f⁻¹⦅y⦆⦆)) (
+                      And.intro (Eq.symm (bij_f_finv f (setPO(𝓐)) (rng f) (hf) x (hx))) (
+                        Eq.symm (bij_f_finv f (setPO(𝓐)) (rng f) (hf) y (hy))
+                      )
+                    )
+                  )
+
+                )
+              ))
+            )
+          )
+        )
+    )
+
+
+
+noncomputable def induced_order (𝓐 f: Set) := ⁅rng f; str (rng f) (induced_R₂ 𝓐 f); (induced_R₂ 𝓐 f)⁆
+
+theorem po_induced : ∀ 𝓐 f X, (f Inj (setPO(𝓐)) To X) → (PartOrd 𝓐) → (PartOrd (induced_order 𝓐 f)) :=
+  fun (𝓐 f X) =>
+    fun (hf) =>
+      fun (h𝓐) =>
+        let B := rng f
+        let R₂ := (induced_R₂ 𝓐 f)
+        let R₁ := str B R₂
+
+        let 𝓑 := ⁅B; R₁; R₂⁆
+        let P := fun (s) => ∃ x y ∈ setPO(𝓐); (x . (≼(𝓐)) . y) ∧ s = (f⦅x⦆, f⦅y⦆)
+
+        let 𝓐nemp := po_emp 𝓐 h𝓐
+        let 𝓐exi := Iff.mp (set_non_empty_iff_non_empty (setPO(𝓐))) 𝓐nemp
+        let rngExi : ∃ y, y ∈ (rng f) := Exists.elim 𝓐exi (
+          fun (x) =>
+            fun (hx) =>
+              Exists.intro (f⦅x⦆) (
+                let u₁ := Iff.mpr (function_equal_value_prop f (setPO(𝓐)) X (And.left hf) x (f⦅x⦆) hx) (Eq.refl (f⦅x⦆))
+
+                Iff.mpr (rng_prop f (f⦅x⦆)) (Exists.intro x (u₁))
+              )
+        )
+        let rngnemp := Iff.mpr (set_non_empty_iff_non_empty (rng f)) rngExi
+        let R₂bin := specification_set_subset P (B × B)
+        let fbij := bij_rng f (setPO(𝓐)) X hf
+        let finvbij := bijection_inv_mp f (setPO(𝓐)) (rng f) fbij
+        let finvfunc := And.left finvbij
+        let finvset := val_in_B (f⁻¹) (rng f) (setPO(𝓐)) finvfunc
+
+        Exists.intro B (
+          Exists.intro R₁ (
+            Exists.intro R₂ (
+              And.intro (Eq.refl 𝓑) (
+                Iff.mpr (part_ord_nspo_crit B R₁ R₂) (
+                  And.intro (rngnemp) (
+                    And.intro (
+
+                      And.intro (R₂bin) (
+
+
+                        And.intro (
+
+                          fun (x) =>
+                            fun (hx) =>
+                              Iff.mpr (induced_crit 𝓐 f fbij x hx x hx) (
+                                refl_R₂ 𝓐 h𝓐 (f⁻¹⦅x⦆) (finvset x (hx))
+                              )
+
+                        ) (And.intro (
+
+                          fun (x) =>
+                            fun (y) =>
+                              fun (hxy) =>
+                                let R₂B := R₂bin (x, y) (And.left hxy)
+                                let cart := Iff.mp (cartesian_product_pair_prop B B x y) R₂B
+                                let u₀ := (Iff.mp (induced_crit 𝓐 f fbij x (And.left cart) y (And.right cart)) (And.left hxy))
+                                let u₁ := (Iff.mp (induced_crit 𝓐 f fbij y (And.right cart) x (And.left cart)) (And.right hxy))
+                                let u₂ := antisymm_R₂ 𝓐 h𝓐 (f⁻¹⦅x⦆) (f⁻¹⦅y⦆) (u₀) (u₁)
+                                let u₃ := And.intro (finvfunc) (And.left (And.right finvbij))
+                                Iff.mp (func_inj_prop (rng f) (setPO(𝓐)) (f⁻¹) finvfunc) u₃ x (
+                                  And.left cart) y (And.right cart) u₂
+
+
+                        ) (
+                          fun (x) =>
+                            fun (y) =>
+                              fun (z) =>
+                                fun (hxyz) =>
+                                  let R₂B₁ := R₂bin (x, y) (And.left hxyz)
+                                  let cart₁ := Iff.mp (cartesian_product_pair_prop B B x y) R₂B₁
+                                  let R₂B₂ := R₂bin (y, z) (And.right hxyz)
+                                  let cart₂ := Iff.mp (cartesian_product_pair_prop B B y z) R₂B₂
+                                  Iff.mpr (induced_crit 𝓐 f fbij x (And.left cart₁) z (And.right cart₂)) (
+                                    trans_R₂ 𝓐 h𝓐 (f⁻¹⦅x⦆) (f⁻¹⦅y⦆) (f⁻¹⦅z⦆) (
+                                      Iff.mp (induced_crit 𝓐 f fbij x (And.left cart₁) y (And.right cart₁)) (
+                                        And.left hxyz
+                                      )
+                                    ) (Iff.mp (induced_crit 𝓐 f fbij y (And.left cart₂) z (And.right cart₂)) (
+                                        And.right hxyz
+                                      ))
+                                  )
+                        ))
+                      )
+
+                    ) (Eq.refl R₁)
+                  )
+                )
+              )
+            )
+          )
+        )
+
+
+theorem poiso_induced : ∀ 𝓐 f X, (PartOrd 𝓐) → (f Inj (setPO(𝓐)) To X) → (f PO_ISO_PO 𝓐 To (induced_order 𝓐 f)) :=
+  fun (𝓐 f X h𝓐 hf) =>
+    And.intro (h𝓐) (
+      And.intro (po_induced 𝓐 f X hf h𝓐) (
+        let B := rng f
+        let R₂ := induced_R₂ 𝓐 f
+        let R₁ := str B R₂
+        let u₁ := setPO_is_setPO B R₁ R₂
+        let u₂ := lesseqPO_is_lesseqPO B R₁ R₂
+        let fbij := bij_rng f (setPO(𝓐)) (X) (hf)
+        And.intro (
+          eq_subst (fun (t) => f Bij (setPO(𝓐)) To t) (B) (setPO(induced_order 𝓐 f)) (Eq.symm u₁) (
+            fbij
+          )
+        ) (
+          let u₃ := induced_crit₀ 𝓐 f fbij
+
+          eq_subst (fun (t) => ∀ x y ∈ (setPO(𝓐)); (x . (≼(𝓐)) . y) ↔ ((f⦅x⦆) . (t) . (f⦅y⦆))) (induced_R₂ 𝓐 f) (≼(induced_order 𝓐 f)) (
+            Eq.symm u₂) (u₃)
+        )
+      )
+    )
