1_SetTheory/3_BinaryRelations/Header/Basic.lean
@@ -33,9 +33,9 @@ macro_rules
   | `(∀ $idnt:ident ∈ $A:term; $b:term)  => `(forall_in_A (fun $idnt:ident => $b) $A)
   | `(∀ $idnt:ident $idnts:idents ∈ $A:term; $b:term) => `(forall_in_A (fun $idnt:ident => (∀ $idnts:idents ∈ $A; $b)) $A)
   | `(∃ $idnt:ident ∈ $A:term; $b:term)  => `(exists_in_A (fun $idnt:ident => $b) $A)
-  | `(∃ $idnt:ident $idnts:idents ∈ $A:term; $b:term) => `(exists_in_A (fun $idnt:ident => (∀ $idnts:idents ∈ $A; $b)) $A)
+  | `(∃ $idnt:ident $idnts:idents ∈ $A:term; $b:term) => `(exists_in_A (fun $idnt:ident => (∃ $idnts:idents ∈ $A; $b)) $A)
   | `(∃! $idnt:ident ∈ $A:term; $b:term)  => `(exists_uniq_in_A (fun $idnt:ident => $b) $A)
-  | `(∃! $idnt:ident $idnts:idents ∈ $A:term; $b:term) => `(exists_uniq_in_A (fun $idnt:ident => (∀ $idnts:idents ∈ $A; $b)) $A)
+  | `(∃! $idnt:ident $idnts:idents ∈ $A:term; $b:term) => `(exists_uniq_in_A (fun $idnt:ident => (∃! $idnts:idents ∈ $A; $b)) $A)
 def empty (A : Set) : Prop := ∀ b, (b ∉ A)
 def non_empty (A : Set) : Prop := ∃ b, (b ∈ A)
 def subset (A B : Set) : Prop := ∀ x ∈ A; x ∈ B
