1_SetTheory/4_Functions/Header/Basic.lean
@@ -43,9 +43,9 @@ macro_rules
   | `(∀ $idnt:ident ∈ $A:term; $b:term)  => `(forall_in_A (fun $idnt:ident => $b) $A)
   | `(∀ $idnt:ident $idnts:idents ∈ $A:term; $b:term) => `(forall_in_A (fun $idnt:ident => (∀ $idnts:idents ∈ $A; $b)) $A)
   | `(∃ $idnt:ident ∈ $A:term; $b:term)  => `(exists_in_A (fun $idnt:ident => $b) $A)
-  | `(∃ $idnt:ident $idnts:idents ∈ $A:term; $b:term) => `(exists_in_A (fun $idnt:ident => (∀ $idnts:idents ∈ $A; $b)) $A)
+  | `(∃ $idnt:ident $idnts:idents ∈ $A:term; $b:term) => `(exists_in_A (fun $idnt:ident => (∃ $idnts:idents ∈ $A; $b)) $A)
   | `(∃! $idnt:ident ∈ $A:term; $b:term)  => `(exists_uniq_in_A (fun $idnt:ident => $b) $A)
-  | `(∃! $idnt:ident $idnts:idents ∈ $A:term; $b:term) => `(exists_uniq_in_A (fun $idnt:ident => (∀ $idnts:idents ∈ $A; $b)) $A)
+  | `(∃! $idnt:ident $idnts:idents ∈ $A:term; $b:term) => `(exists_uniq_in_A (fun $idnt:ident => (∃! $idnts:idents ∈ $A; $b)) $A)
 
 
 def empty (A : Set) : Prop := ∀ b, (b ∉ A)
@@ -266,6 +266,8 @@ syntax  term ".[" term "]" : term
 macro_rules
   | `($R:term .[ $X:term ])  => `(rel_image $X $R)
 
+
+axiom rel_image_id : ∀ A X, (X ⊆ A) → (id_ A).[X] = X
 axiom rel_pre_image_eq : ∀ Y R, (BinRel R) → R⁻¹.[Y] = {a ∈ dom R | ∃ b ∈ Y; (a . R . b)}
 axiom dom_preimage : ∀ A B P, binary_relation_between A B P → dom P = P⁻¹.[B]
 axiom rel_preimage_composition : ∀ P Q X, (BinRel P) → (BinRel Q) → (P ∘ Q)⁻¹.[X] = Q⁻¹.[P⁻¹.[X]]
@@ -279,7 +281,7 @@ axiom union_empty : ⋃ ∅ = ∅
 
 axiom image_prop : ∀ R X y, (y ∈ R.[X] ↔ ∃ x ∈ X; (x . R . y))
 axiom preimage_prop : ∀ R Y, (BinRel R) → ∀ x, (x ∈ R⁻¹.[Y] ↔ ∃ y ∈ Y; (x . R . y))
-
+axiom rel_image_composition : ∀ P Q X, (P ∘ Q).[X] = P.[Q.[X]]
 axiom rel_image_inter : ∀ X Y R, (BinRel R) → R.[X ∩ Y] ⊆ (R.[X] ∩ R.[Y])
 axiom rel_preimage_inter : ∀ X Y R, (BinRel R) → R⁻¹.[X ∩ Y] ⊆ (R⁻¹.[X] ∩ R⁻¹.[Y])
 axiom rel_image_diff : ∀ X Y R, (R.[X] \ R.[Y]) ⊆ (R.[X \ Y])
